Add build system and separate out [expr_denote]

SystemT.v
@@ -17,15 +17,17 @@
  *)
 
 Require List.
-Require Import Relations.
-Import List.ListNotations.
+Export List.ListNotations.
 Open Scope list.
-Require Import Equality.
+
+Require Export Equality.
+
+Require Import Relations.
+Require Import FunctionalExtensionality.
 Require Import Eqdep_dec.
 Require Import Recdef.
-Require Import FunctionalExtensionality.
 
-Set Implicit Arguments.
+Global Set Implicit Arguments.
 
 (** * Language definitions *)
 
@@ -883,76 +885,6 @@ Proof.
   eapply (step_val_unique (e := e));
     eauto using eval_step, eval'_step,
     eval_val, eval'_val.
-Qed.
-
-(** * Some unfinished work on reflecting well-typed terms into Gallina terms. *)
-
-Fixpoint type_denote (t: type) : Type :=
-  match t with
-  | natTy => nat
-  | arrow t1 t2 => type_denote t1 -> type_denote t2
-  end.
-
-Fixpoint ctx_denote (Gamma: context) : Type :=
-  match Gamma with
-  | nil => unit
-  | t :: Gamma' => type_denote t * ctx_denote Gamma'
-  end.
-
-Fixpoint env_get Gamma (env: ctx_denote Gamma)
-         t (v: variable Gamma t) : type_denote t.
-  destruct v.
-  - exact (fst env).
-  - exact (env_get _ (snd env) _ v).
-Defined.
-
-Fixpoint expr_denote Gamma (t: type) (e: expr Gamma t) :
-  ctx_denote Gamma -> type_denote t.
-  intro env.
-  destruct e; simpl; intros.
-  - exact (env_get env v).
-  - exact 0.
-  - exact (S (expr_denote _ _ e env)).
-  - pose proof (expr_denote _ _ e) as f; simpl in *.
-    exact (f (X, env)).
-  - pose proof (expr_denote _ _ e1) as f; simpl in *.
-    pose proof (expr_denote _ _ e2) as x.
-    exact (f env (x env)).
-  - pose proof (expr_denote _ _ e3 env) as n; simpl in n.
-    induction n.
-    exact (expr_denote _ _ e1 env).
-    pose proof (expr_denote _ _ e2) as iter_f; simpl in *.
-    exact (iter_f (IHn, env)).
-Defined.
-
-Lemma expr_denote_step : forall t (e e': expr [] t),
-    e |-> e' ->
-    expr_denote e tt = expr_denote e' tt.
-Proof.
-  induction 1; simpl; intros; eauto; try congruence.
-  - (* TODO: generalize over environments *)
-    admit.
-  - dependent induction H; simplify.
-    (* need general property of expr_denote with for substitutions, not just the
-    shift substitution *)
-    admit.
-    rewrite IHval.
-    admit.
-Admitted.
-
-Lemma expr_denote_step_star : forall t (e e': expr [] t),
-    e |->* e' ->
-    expr_denote e tt = expr_denote e' tt.
-Proof.
-  intros.
-  induction H; auto.
-  pose proof (expr_denote_step H); congruence.
-Qed.
-
-Theorem expr_denote_ok : forall t (e: expr [] t),
-    expr_denote e tt = expr_denote (eval e) tt.
-Proof.
-  eauto using eval_step, expr_denote_step_star.
 Qed.
 
 (* Local Variables: *)
