Makefile
@@ -1,0 +1,14 @@
+default: Makefile.coq
+	$(MAKE) -f Makefile.coq SystemT.vo
+
+all: Makefile.coq
+	$(MAKE) -f Makefile.coq all
+
+Makefile.coq: _CoqProject
+	coq_makefile -f $< -o $@
+
+clean: Makefile.coq
+	$(MAKE) -f Makefile.coq clean
+	rm -f Makefile.coq
+
+.PHONY: all default clean
